Util.v
@@ -1,3 +1,14 @@
+Require Import Coq.Setoids.Setoid.
+
+
+Local Lemma R_refl [A] (R : relation A) (x y : A) (X : R x x) (E : x = y): R x y.
+Proof.
+  rewrite <- E; apply X.
+Qed.
+
+Ltac reflexivityR := apply R_refl; reflexivity.
+
+
 Ltac symmetric_iff :=
   let H  := fresh "H"  in
   eassert _ as H; [|
@@ -10,3 +21,20 @@ Ltac symmetric_iff :=
     clear H Hs
   ].
 
+(* [fset] *)
+
+Definition fset [A B : Type] (e : forall (x y : A), {x=y}+{x<>y}) (x : A) (y : B) (f : A -> B) : A -> B :=
+  fun x' => if e x' x then y else f x'.
+
+Lemma fset_gs [A B] e x y (f : A -> B):
+  fset e x y f x = y.
+Proof.
+  unfold fset; case e; congruence.
+Qed.
+
+Lemma fset_go [A B] e x y (f : A -> B) x'
+  (O : x' <> x):
+  fset e x y f x' = f x'.
+Proof.
+  unfold fset; case e; congruence.
+Qed.
