SLProg.v
@@ -1,0 +1,232 @@
+Require Import SLFun.Util.
+Require Export SLFun.Values.
+Require Import SLFun.SL.
+Require SLFun.ConcreteProg.
+
+Require Import Coq.Setoids.Setoid.
+
+Module CP := ConcreteProg.
+Import SLNotations.
+Open Scope slprop.
+
+Definition match_fmem (f : FMem.t) (m : mem) :=
+  forall p v, f p = Some v -> m p = v.
+
+Definition mem_match_sl (sl : SLprop.t) (m : mem) :=
+  exists fm : FMem.t, match_fmem fm m /\ sl fm.
+
+Lemma mem_match_sl_morph_imp (sl0 sl1 : SLprop.t) (slE : SLprop.imp sl0 sl1) (m : mem):
+  mem_match_sl sl0 m -> mem_match_sl sl1 m.
+Proof.
+  intros (fm & ? & ?); exists fm; auto.
+Qed.
+
+Global Add Morphism mem_match_sl
+  with signature SLprop.eq ==> eq ==> iff
+  as mem_match_sl_morph.
+Proof.
+  symmetric_iff; intros ? ? slE.
+  apply mem_match_sl_morph_imp.
+  rewrite slE; reflexivity.
+Qed.
+
+Module Spec. Section Spec.
+  Local Set Implicit Arguments.
+  Variable A : Type.
+
+  Record t := mk {
+    pre  : SLprop.t;
+    post : A -> SLprop.t;
+  }.
+
+  Definition le (s0 s1 : t) :=
+    SLprop.imp (pre s1) (pre s0) /\ forall x : A, SLprop.imp (post s0 x) (post s1 x).
+
+  Global Instance le_PreOrder : PreOrder le.
+  Proof.
+    unfold le. split.
+    - intro; split; reflexivity.
+    - intros a b c [L0a L0b] [L1a L1b]; split.
+      + rewrite L1a, L0a; reflexivity.
+      + intro; rewrite L0b, L1b; reflexivity.
+  Qed.
+
+  Definition frame (s : t) (fr : SLprop.t) : t := {|
+    pre  := pre s ** fr;
+    post := fun x => post s x ** fr;
+  |}.
+
+  Definition tr (s : t): CP.Spec.t A := {|
+    CP.Spec.pre  := mem_match_sl (pre s);
+    CP.Spec.post := fun _ r => mem_match_sl (post s r);
+  |}.
+
+  Definition wp_match (s : t) (wp : CP.Spec.wp_t A): Prop :=
+    forall fr, CP.Spec.wp_impl wp (tr (frame s fr)).
+
+  Definition spec_match (s : t) (t : CP.Spec.t A -> Prop): Prop :=
+    forall fr, exists t_s, t t_s /\ CP.Spec.le t_s (tr (frame s fr)).
+End Spec. End Spec.
+
+Section F_SPEC.
+  Local Set Implicit Arguments.
+  Variable sg : CP.f_sig.
+
+  Definition f_spec :=
+    CP.f_arg_t sg -> Spec.t (CP.f_ret_t sg) -> Prop.
+
+  Definition match_f_spec (s : f_spec) (t : CP.f_spec sg) : Prop :=
+    forall x s_s, s x s_s -> Spec.spec_match s_s (t x).
+
+  Definition tr_f_spec (s : f_spec) : CP.f_spec sg :=
+    fun x t_s => exists s_s fr, s x s_s /\ t_s = Spec.tr (Spec.frame s_s fr).
+
+  Lemma tr_f_spec_match (s : f_spec):
+    match_f_spec s (tr_f_spec s).
+  Proof.
+    intros x s_s S fr; do 2 esplit.
+    - exists s_s, fr; eauto.
+    - reflexivity.
+  Qed.
+End F_SPEC.
+
+Section SLS.
+  Context [SG : CP.sig_context] (SPC : CP.spec_context SG).
+
+  (* Separation Logic Spec *)
+  Definition sls [A] (i : CP.instr A) (s : Spec.t A) :=
+    Spec.wp_match s (CP.wlp SPC i).
+
+  (* Constructors *)
+
+  Section Ret.
+    Context [A : Type] (x : A) (sp : A -> SLprop.t).
+
+    Definition ret_spec : Spec.t A := {|
+      Spec.pre  := sp x;
+      Spec.post := sp;
+    |}.
+    
+    Lemma Ret : sls (CP.Ret x) ret_spec.
+    Proof.
+      intros fr m0; simpl; auto.
+    Qed.
+  End Ret. 
+  Section Bind.
+    Context [A B : Type]
+      [pre : SLprop.t] [itm : A -> SLprop.t] [post : B -> SLprop.t]
+      [f : CP.instr A] [g : forall x : A, CP.instr B]
+      (Sf : sls f (Spec.mk pre itm)) (Sg : forall x : A, sls (g x) (Spec.mk (itm x) post)).
+
+    Lemma Bind : sls (CP.Bind f (fun x => g x)) (Spec.mk pre post).
+    Proof.
+      intros fr m0; simpl; intros M0.
+      eapply CP.wlp_monotone, Sf, M0.
+      simpl; intros x.
+      apply (Sg x).
+    Qed.
+  End Bind.
+  Section Call.
+    Context [sg : CP.f_sig] (f : CP.fid) (x : CP.f_arg_t sg) (s : Spec.t (CP.f_ret_t sg)).
+    Record fun_has_spec : Prop := {
+      fd_SIG  : SG f = Some sg;
+      fg_SPEC : Spec.spec_match s (CP.fun_has_spec SPC f fd_SIG x);
+    }.
+    Variables (fs : fun_has_spec).
+
+    Lemma Call : sls (CP.Call f (fd_SIG fs) x) s.
+    Proof.
+      intros fr m0; simpl; intro M0.
+      case fs as [SIG SPEC]; simpl.
+      case (SPEC fr) as (t_s & HS & SLE).
+      exists t_s. split. exact HS.
+      exact (SLE _ M0).
+    Qed.
+  End Call.
+  Section Frame.
+    Context [A : Type] (f : CP.instr A) [s : Spec.t A] (Sf : sls f s) (fr : SLprop.t).
+
+    Lemma Frame : sls f (Spec.frame s fr).
+    Proof.
+      intros fr' m0; simpl.
+      setoid_rewrite SLprop.star_assoc at 1.
+      intros M0; eapply CP.wlp_monotone, Sf with (fr := (fr ** fr')); auto.
+      simpl; setoid_rewrite SLprop.star_assoc; auto.
+    Qed.
+  End Frame.
+  Section Cons. 
+    Context [A : Type] (f : CP.instr A) [s0 s1 : Spec.t A] (Sf : sls f s0) (LE : Spec.le s0 s1).
+
+    Lemma Cons : sls f s1.
+    Proof.
+      intros fr m0; simpl; intro M0.
+      eapply CP.wlp_monotone, Sf with (fr := fr); cycle 1; simpl.
+      - eapply mem_match_sl_morph_imp, M0.
+        apply SLprop.star_morph_imp; [apply LE|reflexivity].
+      - intros x m1.
+        apply mem_match_sl_morph_imp, SLprop.star_morph_imp; [apply LE|reflexivity].
+    Qed.
+  End Cons.
+  Section Assert.
+    Variable (P : SLprop.t).
+
+    Definition sl_assert : @CP.instr SG unit :=
+      CP.Assert (fun m => exists fr, mem_match_sl (P ** fr) m).
+
+    Definition assert_spec : Spec.t unit :=
+      Spec.mk P (fun _ => P).
+
+    Lemma Assert : sls sl_assert assert_spec.
+    Proof.
+      intros fr m; simpl; eauto.
+    Qed.
+  End Assert.
+  Section Read.
+    Variables (p : ptr) (d : memdata).
+
+    Definition read_spec : Spec.t memdata := {|
+      Spec.pre  := SLprop.cell p d;
+      Spec.post := fun r => SLprop.cell p d ** SLprop.pure (r = d);
+    |}.
+
+    Lemma Read : sls (CP.Read p) read_spec.
+    Proof.
+      intros fr m; simpl; intro M0.
+      setoid_rewrite SLprop.star_comm at 2.
+      setoid_rewrite SLprop.star_assoc.
+      case M0 as (fm & FM & M0).
+      do 2 esplit. exact FM.
+      exists FMem.emp, fm; intuition.
+      - apply FMem.is_join_emp_r; reflexivity.
+      - split. reflexivity.
+        apply FM.
+        case M0 as (fm_cell & fm_frame & JOIN & CELL & _).
+        simpl in CELL; rewrite CELL in JOIN.
+        specialize (JOIN p); unfold FMem.cell in JOIN.
+        case Mem.ptr_eq in JOIN. 2:congruence.
+        case fm_frame in JOIN; simpl in JOIN; congruence.
+    Qed.
+  End Read.
+  Section Write.
+    Variables (p : ptr) (d0 d1 : memdata).
+
+    Definition write_spec : Spec.t unit := {|
+      Spec.pre  := SLprop.cell p d0;
+      Spec.post := fun _ => SLprop.cell p d1;
+    |}.
+
+    Lemma Write : sls (CP.Write p d1) write_spec.
+    Proof.
+      intros fr m; simpl; intros (fm0 & FM0 & fm_0 & fm_f & J0 & C0 & F0).
+      simpl in C0; rewrite C0 in J0; clear C0 fm_0.
+      exists (fset Mem.ptr_eq p (Some d1) fm0).
+      simpl; split.
+      - intros q d; unfold Mem.write, fset.
+        destruct Mem.ptr_eq. congruence. apply FM0.
+      - exists (FMem.cell p d1), fm_f; intuition.
+        intro q; generalize (J0 q).
+        unfold FMem.cell, fset; case Mem.ptr_eq as [|]; auto.
+        destruct fm_f; simpl; [discriminate 1|reflexivity].
+    Qed.
+  End Write.
+End SLS.
