Test/SLProg.v
@@ -1,0 +1,135 @@
+Require Import SLFun.Util.
+Require Import SLFun.SLProg.
+Require Import SLFun.SL.
+
+Import SLNotations.
+
+
+Definition f_aux  : CP.fid := 0.
+Definition f_main : CP.fid := 1.
+
+Definition sig_aux  := CP.mk_f_sig ptr nat.
+Definition sig_main := CP.mk_f_sig (ptr * ptr) unit.
+
+Definition SIG : CP.sig_context :=
+  fun f => match f with
+  | 0 => Some sig_aux
+  | 1 => Some sig_main
+  | _ => None
+  end.
+
+Definition spec_aux_n (p : ptr) (n : nat) : Spec.t nat := {|
+  Spec.pre  := SLprop.cell p n;
+  Spec.post := fun m => SLprop.cell p (n + m);
+|}.
+
+Definition spec_aux : f_spec sig_aux :=
+  fun p s => exists (n : nat), eq s (spec_aux_n p n).
+
+Definition spec_main_n (ps : ptr * ptr) : Spec.t unit := {|
+  Spec.pre  := SLprop.cell (fst ps) 0 ** SLprop.cell (snd ps) 0;
+  Spec.post := fun _ => SLprop.True;
+|}.
+
+Definition spec_main : f_spec sig_main :=
+  fun ps s => eq s (spec_main_n ps).
+
+Definition SPEC : CP.spec_context SIG :=
+  fun f => match f with
+  | 0 => tr_f_spec spec_aux
+  | 1 => tr_f_spec spec_main
+  | _ => tt
+  end.
+
+Lemma call_aux (p : ptr) (n : nat):
+  @fun_has_spec _ SPEC sig_aux f_aux p (spec_aux_n p n).
+Proof.
+  unshelve eexists. reflexivity.
+  simpl.
+  apply (tr_f_spec_match spec_aux).
+  do 2 esplit.
+Defined.
+
+Definition impl_aux (p : ptr) : @CP.instr SIG nat :=
+  CP.Bind (CP.Read p) (fun n =>
+  CP.Bind (CP.Write p (n + 2)) (fun _ =>
+  CP.Ret 2)).
+
+Lemma sls_aux (p : ptr) (n : nat) : sls SPEC (impl_aux p) (spec_aux_n p n).
+Proof.
+  eapply Bind. eapply Read. intro n'.
+  eapply Cons. eapply Frame with (fr := SLprop.pure (n' = n)).
+  eapply Bind. eapply Write. intro _u.
+  eapply Ret with (sp := fun r => SLprop.cell p (n' + r)).
+  split; simpl.
+  - intros fm H.
+    assert (n' = n). {
+      case H as (? & ? & ? & ? & H); apply H.
+    }
+    subst n'; eassumption.
+  - intro r.
+    rewrite SLprop.star_comm.
+    apply SLprop.imp_pure_l.
+    intros ->; reflexivity.
+Defined.
+
+Definition impl_main (ps : ptr * ptr) : @CP.instr SIG unit :=
+  let (p0, p1) := ps in
+  CP.Bind (CP.Call (sg := sig_aux) f_aux eq_refl p0) (fun n =>
+  CP.Ret tt).
+
+Lemma sls_main ps : sls SPEC (impl_main ps) (spec_main_n ps).
+Proof.
+  case ps as (p0, p1); simpl.
+  eapply Bind.
+  eapply Cons. eapply Frame with (fr := SLprop.cell p1 0).
+  eapply Call with (fs := call_aux p0 0).
+  reflexivityR.
+  intros _n.
+  eapply Cons. exact (Ret _ tt (fun _ => SLprop.True)).
+  split; simpl; constructor.
+Defined.
+
+Definition IMPL : CP.impl_context SIG :=
+  fun f => match f with
+  | 0 => impl_aux
+  | 1 => impl_main
+  | _ => tt
+  end.
+
+Lemma wp_impl_tr_f_spec [sg sp x wp]
+  [IM : Spec.wp_match (sp x) wp]
+  [s] (TR : @tr_f_spec sg (fun x s => s = sp x) x s):
+  CP.Spec.wp_impl wp s.
+Proof.
+  case TR as (? & fr & ? & ?); subst.
+  apply IM.
+Qed.
+
+Lemma tr_f_spec_exists A sg sp x s:
+  @tr_f_spec sg (fun x s => exists y : A, sp s x y) x s ->
+  exists y : A, tr_f_spec (fun x s => sp s x y) x s.
+Proof.
+  intros (? & fr & (y & ?) & ?); subst.
+  eexists y, _, fr; eauto.
+Qed.
+
+Lemma match_context:
+  CP.context_match_spec IMPL SPEC.
+Proof.
+  intros [|[|]]; simpl. 3:constructor.
+  - intros p s TR.
+    apply tr_f_spec_exists in TR as [n TR].
+    refine (wp_impl_tr_f_spec TR).
+    apply sls_aux.
+  - intros ps; apply wp_impl_tr_f_spec.
+    apply sls_main.
+Qed.
+
+Lemma context_oracle_free:
+  CP.context_oracle_free IMPL.
+Proof.
+  intros [|[|]]; simpl; repeat constructor.
+  (* intro. set (imp := impl_main x); hnf in imp; subst imp. *)
+  intros (?,?); simpl; repeat constructor.
+Qed.
